more code preparation

Weidenbach_Book/CDCL_Conflict_Minimisation.thy
@@ -263,6 +263,16 @@ qed
 
 datatype minimize_status = SEEN_FAILED | SEEN_REMOVABLE | SEEN_UNKNOWN
 
+instance minimize_status :: heap
+proof standard
+  let ?f = \<open>\<lambda>s. case s of SEEN_FAILED \<Rightarrow> (0 :: nat) | SEEN_REMOVABLE \<Rightarrow> 1 | SEEN_UNKNOWN \<Rightarrow> 2\<close>
+  have \<open>inj ?f\<close>
+    by (auto simp: inj_def split: minimize_status.splits)
+  then show \<open>\<exists>to_nat. inj (to_nat :: minimize_status \<Rightarrow> nat)\<close>
+    by blast
+qed
+
+
 type_synonym 'v conflict_min_analyse = \<open>('v literal \<times> 'v clause) list\<close>
 type_synonym 'v conflict_min_cach = \<open>'v \<Rightarrow> minimize_status\<close>
 
@@ -1162,7 +1172,7 @@ where
   \<open>mark_failed_lits_wl analyse cach = SPEC(\<lambda>cach'.
      (\<forall>L. cach' L = SEEN_REMOVABLE \<longrightarrow> cach L = SEEN_REMOVABLE))\<close>
 
-context isasat_input_bounded
+context isasat_input_ops
 begin
 
 definition lit_redundant_rec_wl :: \<open>('v, nat) ann_lits \<Rightarrow> 'v clauses_l \<Rightarrow> 'v clause \<Rightarrow>
@@ -1639,19 +1649,131 @@ proof -
     done
 qed
 
-abbreviation (in -)  minimize_status_rel where
+abbreviation (in -) minimize_status_rel where
   \<open>minimize_status_rel \<equiv> Id :: (minimize_status \<times> minimize_status) set\<close>
 
-definition cach_refinement :: \<open>(minimize_status list \<times> (nat conflict_min_cach)) set\<close>  where
-  \<open>cach_refinement = \<langle>Id\<rangle>map_fun_rel {(a, a'). a = a \<and> a \<in># \<A>\<^sub>i\<^sub>n}\<close>
+abbreviation (in -) minimize_status_assn where
+  \<open>minimize_status_assn \<equiv> (id_assn :: minimize_status\<Rightarrow> _)\<close>
+
+lemma (in -) SEEN_REMOVABLE[sepref_fr_rules]:
+  \<open>(uncurry0 (return SEEN_REMOVABLE),uncurry0 (RETURN SEEN_REMOVABLE)) \<in>
+     unit_assn\<^sup>k \<rightarrow>\<^sub>a minimize_status_assn\<close>
+  by (sepref_to_hoare) sep_auto
+
+lemma (in -) SEEN_FAILED[sepref_fr_rules]:
+  \<open>(uncurry0 (return SEEN_FAILED),uncurry0 (RETURN SEEN_FAILED)) \<in>
+     unit_assn\<^sup>k \<rightarrow>\<^sub>a minimize_status_assn\<close>
+  by (sepref_to_hoare) sep_auto
+
+lemma (in -) SEEN_UNKNOWN[sepref_fr_rules]:
+  \<open>(uncurry0 (return SEEN_UNKNOWN),uncurry0 (RETURN SEEN_UNKNOWN)) \<in>
+     unit_assn\<^sup>k \<rightarrow>\<^sub>a minimize_status_assn\<close>
+  by (sepref_to_hoare) sep_auto
+
+definition cach_refinement_list :: \<open>(minimize_status list \<times> (nat conflict_min_cach)) set\<close>  where
+  \<open>cach_refinement_list = \<langle>Id\<rangle>map_fun_rel {(a, a'). a = a' \<and> a \<in># \<A>\<^sub>i\<^sub>n}\<close>
+
+definition cach_refinement_nonull :: \<open>((minimize_status list \<times> nat list) \<times> minimize_status list) set\<close>  where
+  \<open>cach_refinement_nonull = {((cach, support), cach'). cach = cach' \<and>
+       (\<forall>L < length cach. cach ! L \<noteq> SEEN_UNKNOWN \<longrightarrow> L \<in> set support)}\<close>
+
+definition cach_refinement :: \<open>((minimize_status list \<times> nat list) \<times> (nat conflict_min_cach)) set\<close>  where
+  \<open>cach_refinement = cach_refinement_nonull O cach_refinement_list\<close>
+
+abbreviation (in -) cach_refinement_l_assn where
+  \<open>cach_refinement_l_assn \<equiv> array_assn minimize_status_assn *assn arl_assn nat_assn\<close>
+
+definition cach_refinement_assn where
+  \<open>cach_refinement_assn = hr_comp cach_refinement_l_assn cach_refinement\<close>
+
+lemma cach_refinement_alt_def:
+  \<open>((cach, support), cach') \<in> cach_refinement \<longleftrightarrow>
+     (cach, cach') \<in> cach_refinement_list \<and> (\<forall>L<length cach. cach ! L \<noteq> SEEN_UNKNOWN \<longrightarrow> L \<in> set support)\<close>
+  by (auto simp: cach_refinement_def cach_refinement_nonull_def cach_refinement_list_def)
+
+type_synonym (in -) conflict_min_cach_l = \<open>minimize_status list \<times> nat list\<close>
 
 definition (in -) conflict_min_cach :: \<open>nat conflict_min_cach \<Rightarrow> nat \<Rightarrow> minimize_status\<close> where
   [simp]: \<open>conflict_min_cach cach L = cach L\<close>
 
+definition (in -) conflict_min_cach_l :: \<open>conflict_min_cach_l \<Rightarrow> nat \<Rightarrow> minimize_status nres\<close> where
+  \<open>conflict_min_cach_l = (\<lambda>(cach, sup) L. do {
+     ASSERT(L < length cach);
+     RETURN (cach ! L)
+   })\<close>
+
+sepref_definition (in -) conflict_min_cach_l_code
+  is \<open>uncurry conflict_min_cach_l\<close>
+  :: \<open>cach_refinement_l_assn\<^sup>k *\<^sub>a nat_assn\<^sup>k \<rightarrow>\<^sub>a minimize_status_assn\<close>
+  unfolding conflict_min_cach_l_def
+  by sepref
+
 lemma nth_conflict_min_cach:
-  \<open>(uncurry (RETURN oo nth), uncurry (RETURN oo conflict_min_cach)) \<in>
+  \<open>(uncurry conflict_min_cach_l, uncurry (RETURN oo conflict_min_cach)) \<in>
      [\<lambda>(cach, L). L \<in># \<A>\<^sub>i\<^sub>n]\<^sub>f cach_refinement \<times>\<^sub>r nat_rel \<rightarrow> \<langle>minimize_status_rel\<rangle>nres_rel\<close>
-  by (intro frefI nres_relI) (auto simp: cach_refinement_def map_fun_rel_def)
+  by (intro frefI nres_relI) (auto simp: cach_refinement_def map_fun_rel_def
+      cach_refinement_nonull_def cach_refinement_list_def conflict_min_cach_l_def)
+
+lemma conflict_min_cach_hnr[sepref_fr_rules]:
+  \<open>(uncurry conflict_min_cach_l_code, uncurry (RETURN \<circ>\<circ> conflict_min_cach))
+   \<in> [\<lambda>(a, b). b \<in># \<A>\<^sub>i\<^sub>n]\<^sub>a cach_refinement_assn\<^sup>k *\<^sub>a nat_assn\<^sup>k \<rightarrow> minimize_status_assn\<close>
+  using conflict_min_cach_l_code.refine[FCOMP nth_conflict_min_cach,
+     unfolded cach_refinement_assn_def[symmetric]] .
+
+definition (in -) conflict_min_cach_set_failed
+   :: \<open>nat conflict_min_cach \<Rightarrow> nat \<Rightarrow> nat conflict_min_cach\<close>
+where
+  [simp]: \<open>conflict_min_cach_set_failed cach L = cach(L := SEEN_FAILED)\<close>
+
+definition (in -) conflict_min_cach_set_failed_l
+  :: \<open>conflict_min_cach_l \<Rightarrow> nat \<Rightarrow> conflict_min_cach_l nres\<close>
+where
+  \<open>conflict_min_cach_set_failed_l = (\<lambda>(cach, sup) L. do {
+     ASSERT(L < length cach);
+     RETURN (cach[L := SEEN_FAILED], sup @ [L])
+   })\<close>
+
+lemma conflict_min_cach_set_failed:
+  \<open>(uncurry conflict_min_cach_set_failed_l, uncurry (RETURN oo conflict_min_cach_set_failed)) \<in>
+     [\<lambda>(cach, L). L \<in># \<A>\<^sub>i\<^sub>n]\<^sub>f cach_refinement \<times>\<^sub>r nat_rel \<rightarrow> \<langle>cach_refinement\<rangle>nres_rel\<close>
+  by (intro frefI nres_relI)
+     (auto simp: cach_refinement_alt_def map_fun_rel_def  cach_refinement_list_def
+      conflict_min_cach_set_failed_l_def)
+
+
+definition (in -) conflict_min_cach_set_removable
+  :: \<open>nat conflict_min_cach \<Rightarrow> nat \<Rightarrow> nat conflict_min_cach\<close>
+where
+  [simp]: \<open>conflict_min_cach_set_removable cach L = cach(L:= SEEN_REMOVABLE)\<close>
+
+definition (in -) conflict_min_cach_set_removable_l
+  :: \<open>conflict_min_cach_l \<Rightarrow> nat \<Rightarrow> conflict_min_cach_l nres\<close>
+where
+  \<open>conflict_min_cach_set_removable_l = (\<lambda>(cach, sup) L. do {
+     ASSERT(L < length cach);
+     RETURN (cach[L := SEEN_REMOVABLE], sup @ [L])
+   })\<close>
+
+sepref_definition (in -) conflict_min_cach_set_removable_l_code
+  is \<open>uncurry conflict_min_cach_set_removable_l\<close>
+  :: \<open>cach_refinement_l_assn\<^sup>d *\<^sub>a nat_assn\<^sup>k \<rightarrow>\<^sub>a cach_refinement_l_assn\<close>
+  unfolding conflict_min_cach_set_removable_l_def
+  by sepref
+
+lemma conflict_min_cach_set_removable:
+  \<open>(uncurry conflict_min_cach_set_removable_l,
+    uncurry (RETURN oo conflict_min_cach_set_removable)) \<in>
+     [\<lambda>(cach, L). L \<in># \<A>\<^sub>i\<^sub>n]\<^sub>f cach_refinement \<times>\<^sub>r nat_rel \<rightarrow> \<langle>cach_refinement\<rangle>nres_rel\<close>
+  by (intro frefI nres_relI)
+     (auto simp: cach_refinement_alt_def map_fun_rel_def  cach_refinement_list_def
+      conflict_min_cach_set_removable_l_def)
+
+lemma conflict_min_cach_set_removable_hnr[sepref_fr_rules]:
+   \<open>(uncurry conflict_min_cach_set_removable_l_code,
+        uncurry (RETURN \<circ>\<circ> conflict_min_cach_set_removable))
+    \<in> [\<lambda>(a, b). b \<in># \<A>\<^sub>i\<^sub>n]\<^sub>a cach_refinement_assn\<^sup>d *\<^sub>a nat_assn\<^sup>k \<rightarrow> cach_refinement_assn\<close>
+  using conflict_min_cach_set_removable_l_code.refine[FCOMP conflict_min_cach_set_removable,
+    unfolded cach_refinement_assn_def[symmetric]] .
 
 end
 
